Implement a decision procedure for frame_agree_perms
The challenge is to show the decidability of a predicate of the form
(forall o k p, perm m b o k p -> P o).

This is challenging because the o is a Z, therefore unbounded.
If we keep in the memory some information about the range of offsets
that may have permissions, this becomes decidable because all we have
to enumerate is that specific range.

This is implemented as a [mem_bounds] field of the memory implementation,
which associates with each block a range [lo,hi] of offsets where we /may/
have permissions. Those permissions may be dropped at some later point in
the program.

Prior to this commit, we needed to have a specific implementation of
[record_stack_blocks_none] which took as a parameter a proof that all
the offsets with permissions in the blocks of the frame that we try to
record indeed satisfied `P` (in the example above), i.e. it had to be in
the bounds of the frame itself.

With this commit, it will become useless to have both inductive and
operational definitions of [record_stack_blocks].

common/Memimpl.v
@@ -93,7 +93,6 @@ Section FORALL.
 
 End FORALL.
 
-
 Local Notation "a # b" := (PMap.get b a) (at level 1).
 
 Module Mem.
@@ -1117,49 +1116,131 @@ Inductive record_stack_blocks (m: mem) (f: frame_adt) : mem -> Prop :=
                          (mem_bounds m)
                          (mem_bounds_perm m)).
 
-Program Definition record_stack_blocks_none (m: mem) bl sz
-        (RNG: Forall (fun b => forall o k p, Mem.perm m (fst b) o k p ->
-                                     0 <= o < frame_size (snd b))%Z bl)
-  : option mem :=
-  if (Forall_dec _ (fun b => valid_block_dec m (fst b)) bl)
-  then if (Forall_dec _ (fun x => sumbool_not (in_frames_dec (stack_adt m) (fst x))) bl)
-       then if (zlt (size_stack (stack_adt m) + align (Z.max 0 sz) 8) stack_limit)
-            then if (list_norepet_dec peq (map fst bl))
-                 then Some
-                        (mkmem (mem_contents m)
-                               (mem_access m)
-                               (nextblock m)
-                               (access_max m)
-                               (nextblock_noaccess m)
-                               (contents_default m)
-                               ({| frame_adt_blocks := bl;
-                                   frame_adt_size := sz |} :: stack_adt m)
-                               (valid_frames_add _ _ _ (stack_valid m) _)
-                               (nodup_add _ _ (stack_norepet m) _)
-                               (frame_agree_perms_add _ _ _ (stack_perm m) _)
-                               (size_stack_add _ _ _)
-                               (mem_bounds m)
-                               _)
+Definition frame_agree_perms_forall (P: block -> Z -> perm_kind -> permission -> Prop) f :=
+  Forall (fun bfi =>
+            let '(b,fi) := bfi in
+            forall o k p,
+              P b o k p -> 0 <= o < frame_size fi
+         )(frame_adt_blocks f).
+
+Lemma frame_agree_perms_rew:
+  forall P f,
+    frame_agree_perms P f <-> frame_agree_perms_forall P f.
+Proof.
+  unfold frame_agree_perms, frame_agree_perms_forall; split; intros; rewrite ? Forall_forall in *; intros.
+  - destruct x as [b fi]; intros; eauto.
+  - eapply H in H0; eapply H0; eauto.
+Qed.
+
+
+Definition dec (P: Prop) := {P} + {~ P}.
+
+Lemma dec_eq:
+  forall (P Q: Prop) (EQ: P <-> Q), dec P -> dec Q.
+Proof.
+  intros P Q EQ D.
+  destruct D; [left|right]; tauto.
+Qed.
+
+Lemma dec_impl:
+  forall (A: Type) (P Q R: A -> Prop)
+    (IMPL: forall x, P x -> Q x)
+    (DECR: dec (forall x, Q x -> P x -> R x)),
+    dec (forall x, P x -> R x).
+Proof.
+  intros A P Q R IMPL.
+  apply dec_eq.
+  split; intros; eauto.
+Qed.
+
+Definition zle_zlt_dec:
+  forall (a b c: Z), {a <= b < c} + { ~ a <= b < c }.
+Proof.
+  intros a b c; destruct (zle a b), (zlt b c);[left; omega|right; omega..].
+Qed.
+
+Definition frame_agree_perms_forall_dec m f:
+  {frame_agree_perms_forall (perm m) f} + { ~ frame_agree_perms_forall (perm m) f}.
+Proof.
+  apply Forall_dec. intros [b fi].
+  apply dec_eq with (P := Forall (fun k => forall o p, perm m b o k p -> 0 <= o < frame_size fi) (Cur::Max::nil)).
+  {
+    rewrite Forall_forall.
+    split; intros; eauto.
+    eapply H; eauto.
+    destruct k; simpl; auto.
+  }
+  apply Forall_dec. intro k.
+  apply dec_eq with (P := Forall (fun p => forall o, perm m b o k p -> 0 <= o < frame_size fi) (Nonempty::Readable::Writable::Freeable::nil)).
+  {
+    rewrite Forall_forall.
+    split; intros; eauto.
+    eapply H; eauto.
+    destruct p; simpl; auto.
+  }
+  apply Forall_dec. intro p.
+  set (P := fun o : Z => perm m b o k p).
+  set (Q := fun o => in_bounds o (mem_bounds m) # b).
+  set (R := fun o => 0 <= o < frame_size fi).
+  apply (dec_impl _ P Q R).
+  - unfold P, Q. intros; eapply mem_bounds_perm; eauto.
+  - unfold dec, Q. unfold in_bounds. apply forall_rec.
+    intro o. unfold P, R.
+    destruct (zle_zlt_dec 0 o (frame_size fi)).
+    + left; auto.
+    + destruct (perm_dec m b o k p); auto.
+      left; intuition.
+Defined.
+
+Definition frame_agree_perms_dec m f:
+  {frame_agree_perms (perm m) f} + { ~ frame_agree_perms (perm m) f}.
+Proof.
+  destruct (frame_agree_perms_forall_dec m f); rewrite <- frame_agree_perms_rew in *; eauto.
+Defined.
+
+Program Definition record_stack_blocks_exec (m: mem) (f: frame_adt) : option mem :=
+  if (Forall_dec _ (fun b => valid_block_dec m (fst b)) (frame_adt_blocks f))
+  then if (Forall_dec _ (fun x => sumbool_not (in_frames_dec (stack_adt m) (fst x))) (frame_adt_blocks f))
+       then if (zlt (size_stack (stack_adt m) + align (Z.max 0 (frame_adt_size f)) 8) stack_limit)
+            then if (list_norepet_dec peq (map fst (frame_adt_blocks f)))
+                 then if frame_agree_perms_forall_dec m f
+                      then Some
+                             (mkmem (mem_contents m)
+                                    (mem_access m)
+                                    (nextblock m)
+                                    (access_max m)
+                                    (nextblock_noaccess m)
+                                    (contents_default m)
+                                    (f :: stack_adt m)
+                                    (valid_frames_add _ _ _ (stack_valid m) _)
+                                    (nodup_add _ _ (stack_norepet m) _)
+                                    (frame_agree_perms_add _ _ _ (stack_perm m) _)
+                                    (size_stack_add _ _ _)
+                                    (mem_bounds m)
+                                    _)
+                      else None
                  else None
             else None
        else None
   else None.
 Next Obligation.
-  red in H3. simpl in H3.
-  rewrite Forall_forall in H. rewrite in_map_iff in H3.
-  destruct H3 as ((bb,fi) & EQ & IN).
+  red in H4. simpl in H4.
+  rewrite Forall_forall in H. rewrite in_map_iff in H4.
+  destruct H4 as ((bb,fi) & EQ & IN).
   apply H in IN. subst; simpl in *; auto.
 Qed.
 Next Obligation.
   rewrite Forall_forall in H0 |- *.
-  intros. rewrite in_map_iff in H3.
-  destruct H3 as ((bb,fi) & EQ & IN).
+  intros. rewrite in_map_iff in H4.
+  destruct H4 as ((bb,fi) & EQ & IN).
   apply H0 in IN. subst; simpl in *; auto.
+Qed.
+Next Obligation.
+  revert H3. eapply Forall_impl. intros [b fi]. simpl; auto.
 Qed.
 Next Obligation.
   eapply mem_bounds_perm; eauto.
 Qed.
-
 Lemma record_stack_blocks_ext:
   forall m1 fi m2 m2',
     record_stack_blocks m1 fi m2 ->
@@ -1169,6 +1250,39 @@ Proof.
   intros; subst; congruence.
 Qed.
 
+Lemma record_stack_blocks_exec_correct:
+  forall m fa m',
+    record_stack_blocks_exec m fa = Some m' <->
+    record_stack_blocks m fa m'.
+Proof.
+  unfold record_stack_blocks_exec.
+  split; intros.
+  - repeat destr_in H; try congruence.
+    eapply record_stack_blocks_ext. econstructor. apply mkmem_ext; auto.
+  - inv H.
+    repeat destr.
+    + f_equal. apply mkmem_ext; auto.
+    + exfalso; apply n.
+      revert RNG; apply Forall_impl. intros [b fi]; simpl; auto.
+    + exfalso; apply n. destruct fa; auto.
+    + exfalso; apply n.
+      rewrite Forall_forall in NOTIN |- *. intros; eapply NOTIN.
+      apply in_map. auto.
+    + exfalso; apply n.
+      red in VF.
+      rewrite Forall_forall. intros [b fi]. simpl; intro IN. apply VF.
+      eapply in_frame_blocks_in_frame; eauto.
+    Unshelve.
+    auto.
+    revert f1; apply Forall_impl. intros [b fi]; simpl; auto.
+    rewrite Forall_forall in f0 |- *. intros.
+    rewrite in_map_iff in H. destruct H as ((bb&ff) & EQ & IN). simpl in *; subst.
+    intros; eapply f0 in IN. auto.
+    red; simpl; intros. rewrite Forall_forall in f.
+    edestruct in_frame_info as (fi & IN); eauto. simpl in IN.
+    apply f in IN. auto.
+Qed.
+
 Lemma record_stack_blocks_ext':
   forall m1 fi fi' m2,
     record_stack_blocks m1 fi m2 ->
@@ -1176,41 +1290,6 @@ Lemma record_stack_blocks_ext':
     record_stack_blocks m1 fi' m2.
 Proof.
   intros; subst; congruence.
-Qed.
-
-
-Lemma record_stack_blocks_none_correct:
-  forall m bl sz m',
-  (exists pf, record_stack_blocks_none m bl sz pf = Some m') <->
-  (exists fa, record_stack_blocks m fa m' /\ frame_adt_blocks fa = bl /\ frame_adt_size fa = sz).
-Proof.
-  unfold record_stack_blocks_none.
-  split; intros.
-  - repeat destr_in H; try congruence.
-    eexists; split. eapply record_stack_blocks_ext. econstructor. inv H0. apply mkmem_ext; auto.
-    split; reflexivity. 
-  - destruct H as (fa & RSB & BLOCKS & SIZE). subst. inv RSB.
-    exists RNG.
-    repeat destr. f_equal. apply mkmem_ext; auto.
-    f_equal. destruct fa. simpl. f_equal. apply proof_irr.
-    exfalso; apply n; destruct fa; auto.
-    exfalso; apply n.
-    rewrite Forall_forall in NOTIN |- *. intros; eapply NOTIN.
-    apply in_map. auto.
-    exfalso; apply n.
-    red in VF.
-    rewrite Forall_forall; intros. destruct x. apply VF. simpl.
-    eapply in_frame_blocks_in_frame; eauto.
-    Unshelve.
-    + red; simpl; intros. rewrite Forall_forall in f.
-      edestruct in_frame_info as (fi & IN); eauto. simpl in IN.
-      apply f in IN. auto.
-    + simpl. 
-      rewrite Forall_forall in f0 |- *. intros.
-      rewrite in_map_iff in H. destruct H as ((bb&ff) & EQ & IN). simpl in *; subst.
-      intros; eapply f0 in IN. auto.
-    + simpl. auto.
-    + simpl. auto.
 Qed.
 
 Fixpoint do_stores (m: mem) (l: list (memory_chunk * val * val)) : option mem :=
@@ -1664,7 +1743,7 @@ Proof.
   exact storebytes.
   exact drop_perm.
   exact nextblock.
-  (* exact perm. *)
+  exact perm.
   exact valid_pointer.
   exact @extends.
   exact @magree.
@@ -1675,7 +1754,7 @@ Proof.
   exact stack_adt.
   exact record_stack_blocks.
   exact push_frame.
-  exact record_stack_blocks_none.
+  exact record_stack_blocks_exec.
   exact unrecord_stack_block.
   exact stack_limit.
   (* exact update_top_stack_adt. *)
@@ -8740,7 +8819,7 @@ Proof.
   intros. simpl. eapply stack_below_limit.
   apply push_frame_alloc_record.
   apply alloc_record_push_frame.
-  apply record_stack_blocks_none_correct.
+  apply record_stack_blocks_exec_correct.
   intros; eapply record_stack_block_inject_left_zero; eauto.
   intros; eapply unrecord_stack_block_inject_left_zero; eauto.
   intros; eapply mem_inject_ext; eauto.
